common/Values.v
@@ -2580,6 +2580,10 @@ Notation meminj := Val.meminj.
 Definition inject_incr (f1 f2: meminj) : Prop :=
   forall b b' delta, f1 b = Some(b', delta) -> f2 b = Some(b', delta).
 
+Definition incr_without_glob (j j' : meminj) : Prop :=
+  forall b b' delta, j b = None -> j' b = Some (b',delta) ->
+       is_stack b /\ is_stack b'.
+
 Lemma inject_incr_refl :
    forall f , inject_incr f f .
 Proof. unfold inject_incr. auto. Qed.
