driver/Compiler.v
@@ -35,10 +35,8 @@ Require Cshmgen.
 Require Cminorgen.
 Require Selection.
 Require RTLgen.
-(*
 Require Tailcall.
 Require Inlining.
-*)
 Require Renumber.
 Require Constprop.
 Require CSE.
@@ -58,10 +56,8 @@ Require Cshmgenproof.
 Require Cminorgenproof.
 Require Selectionproof.
 Require RTLgenproof.
-(*
 Require Tailcallproof.
 Require Inliningproof.
-*)
 Require Renumberproof.
 Require Constpropproof.
 Require CSEproof.
@@ -124,10 +120,9 @@ Definition partial_if {A: Type}
 Definition transf_rtl_program (f: RTL.program) : res Asm.program :=
    OK f
    @@ print (print_RTL 0)
-(*
    @@ total_if Compopts.optim_tailcalls (time "Tail calls" Tailcall.transf_program)
    @@ print (print_RTL 1)
-  @@@ time "Inlining" Inlining.transf_program *)
+  @@@ time "Inlining" Inlining.transf_program
    @@ print (print_RTL 2)
    @@ time "Renumbering" Renumber.transf_program
    @@ print (print_RTL 3)
@@ -240,10 +235,8 @@ Definition CompCert's_passes :=
   ::: mkpass Cminorgenproof.match_prog
   ::: mkpass Selectionproof.match_prog
   ::: mkpass RTLgenproof.match_prog
-(*
   ::: mkpass (match_if Compopts.optim_tailcalls Tailcallproof.match_prog)
   ::: mkpass Inliningproof.match_prog
-*)
   ::: mkpass Renumberproof.match_prog
   ::: mkpass (match_if Compopts.optim_constprop Constpropproof.match_prog)
   ::: mkpass (match_if Compopts.optim_constprop Renumberproof.match_prog)
@@ -285,11 +278,9 @@ Proof.
   destruct (Selection.sel_program p4) as [p5|e] eqn:P5; simpl in T; try discriminate.
   destruct (RTLgen.transl_program p5) as [p6|e] eqn:P6; simpl in T; try discriminate.
   unfold transf_rtl_program, time in T. rewrite ! compose_print_identity in T. simpl in T.
-(*
   set (p7 := total_if optim_tailcalls Tailcall.transf_program p6) in *.
   destruct (Inlining.transf_program p7) as [p8|e] eqn:P8; simpl in T; try discriminate.
-*)
-  set (p9 := Renumber.transf_program p6) in *.
+  set (p9 := Renumber.transf_program p8) in *.
   set (p10 := total_if optim_constprop Constprop.transf_program p9) in *.
   set (p11 := total_if optim_constprop Renumber.transf_program p10) in *.
   destruct (partial_if optim_CSE CSE.transf_program p11) as [p12|e] eqn:P12; simpl in T; try discriminate.
@@ -308,9 +299,8 @@ Proof.
   exists p4; split. apply Cminorgenproof.transf_program_match; auto.
   exists p5; split. apply Selectionproof.transf_program_match; auto.
   exists p6; split. apply RTLgenproof.transf_program_match; auto.
-(*
   exists p7; split. apply total_if_match. apply Tailcallproof.transf_program_match.
-  exists p8; split. apply Inliningproof.transf_program_match; auto. *)
+  exists p8; split. apply Inliningproof.transf_program_match; auto.
   exists p9; split. apply Renumberproof.transf_program_match; auto.
   exists p10; split. apply total_if_match. apply Constpropproof.transf_program_match.
   exists p11; split. apply total_if_match. apply Renumberproof.transf_program_match.
@@ -374,7 +364,7 @@ Ltac DestructM :=
       destruct H as (p & M & MM); clear H
   end.
   repeat DestructM. subst tp.
-  assert (F: forward_simulation (Cstrategy.semantics p) (Asm.semantics p19)).
+  assert (F: forward_simulation (Cstrategy.semantics p) (Asm.semantics p21)).
   {
   eapply compose_forward_simulations.
     eapply SimplExprproof.transl_program_correct; eassumption.
@@ -388,12 +378,10 @@ Ltac DestructM :=
     eapply Selectionproof.transf_program_correct; eassumption.
   eapply compose_forward_simulations.
     eapply RTLgenproof.transf_program_correct; eassumption.
-(*
   eapply compose_forward_simulations.
     eapply match_if_simulation. eassumption. exact Tailcallproof.transf_program_correct.
   eapply compose_forward_simulations.
     eapply Inliningproof.transf_program_correct; eassumption.
-*)
   eapply compose_forward_simulations. eapply Renumberproof.transf_program_correct; eassumption.
   eapply compose_forward_simulations.
     eapply match_if_simulation. eassumption. exact Constpropproof.transf_program_correct.
